\begin{solution}{Question 5.1}\label{ques:5.1}
    \begin{question}
    Consider an operator that maps a matrix $\bfM \in \C^{2\times 2}$ to \\
    $\frac{1}{4}(\bfM + \bfX \cdot \bfM \cdot \bfX + \bfZ \cdot \bfM \cdot \bfZ+ \bfX \cdot \bfZ \cdot \bfM \cdot \bfZ \cdot \bfX$.\\
    What is the output when this operator is applied to $\bfM \in \{\bfI, \bfX, \bfZ, \bfX \cdot \bfZ\}$?
    \end{question}
    \tcblower{}
    \begin{proof}
    The outputs for different values for M are as follows:
    \begin{enumerate}
        \item $\bfM = \bfI$
        \begin{equation}
            \begin{split}
                f(\bfI) &=\frac{1}{4}(\bfI + \bfX \cdot \bfI \cdot \bfX + \bfZ \cdot \bfI \cdot \bfZ+ \bfX \cdot \bfZ \cdot \bfI \cdot \bfZ \cdot \bfX)\\
                &=\frac{1}{4}(\bfI+\bfI+\bfI+\bfI)\\
                &=\bfI
            \end{split}
        \end{equation}
        \item $\bfM = \bfX$
        \begin{equation}
            \begin{split}
                f(\bfX) &=\frac{1}{4}(\bfX + \bfX \cdot \bfX \cdot \bfX + \bfZ \cdot \bfX \cdot \bfZ+ \bfX \cdot \bfZ \cdot \bfX \cdot \bfZ \cdot \bfX)\\
                &=\frac{1}{4}(\bfX + \bfX - \bfX -\bfX)\\
                &=\mathbf{0}
            \end{split}
        \end{equation}
        \item $\bfM = \bfZ$
        \begin{equation}
            \begin{split}
                f(\bfZ) &=\frac{1}{4}(\bfZ + \bfX \cdot \bfZ \cdot \bfX + \bfZ \cdot \bfZ \cdot \bfZ+ \bfX \cdot \bfZ \cdot \bfZ \cdot \bfZ \cdot \bfX)\\
                &=\frac{1}{4}(\bfZ - \bfZ + \bfZ- \bfZ)\\
                &=\mathbf{0}
            \end{split}
        \end{equation}
        \item $\bfM = \bfX \cdot \bfZ$
        \begin{equation}
            \begin{split}
                f(\bfX\cdot\bfZ) &=\frac{1}{4}(\bfX \cdot \bfZ + \bfX \cdot \bfX \cdot \bfZ \cdot \bfX + \bfZ \cdot \bfX \cdot \bfZ \cdot \bfZ+ \bfX \cdot (\bfZ \cdot \bfX \cdot \bfZ) \cdot \bfZ \cdot \bfX)\\
                &=\frac{1}{4}(\bfX \cdot \bfZ + \bfX \cdot (-\bfZ) + (-\bfX) \cdot \bfZ+ \bfX \cdot (-\bfX \cdot \bfZ\cdot \bfX))\\
                &=\frac{1}{4}(\bfX \cdot \bfZ - \bfX \cdot \bfZ -\bfX \cdot \bfZ+ \bfX \cdot \bfZ)\\
                &=\mathbf{0}
            \end{split}
        \end{equation}
    \end{enumerate}
    
    \end{proof}
\end{solution}
